src/InsertionSort.v
@@ -1,0 +1,186 @@
+From Coq Require Import List Arith Psatz.
+
+From Clairvoyance Require Import Core Approx List ListA Tick Misc.
+
+Import ListNotations.
+Import Tick.Notations.
+
+Module CaseStudyInsert.
+
+Import CaseStudyFolds.
+
+Definition insertA_pessim_ :
+(** The pessimistic specification of [insertA_]. *)
+forall (xs : list nat) (xsA : (listA nat)) (v : nat),
+  xsA `is_approx` xs ->  
+  (insertA_ v xsA)
+    {{ fun zsA cost => cost <= 2 * length xs }}.
+Proof.
+  intros. revert xsA H.
+  induction xs; intros.
+  - mgo_list.
+  - mgo_list. 
+    destruct (v <=? exact a) eqn:LE.
+    + mgo_. subst. inv H4.
+      relax_apply IHxs; eauto.
+      intros xs' n L.
+      mgo_.
+    + mgo_. 
+Qed.
+
+Definition insertA_pessim :
+(** The pessimistic specification of [foldrA]. *)
+forall (xs : list nat) (xsA : T (listA nat)) (vA : T nat) (v : nat),
+  vA `is_approx` v ->
+  xsA `is_approx` xs ->  
+  (insertA vA xsA)
+    {{ fun zsA cost => cost <= 2 * length xs + 2 }}.
+Proof.
+  intros xs xsA. 
+  destruct xsA; unfold insertA; [|mgo_list].
+  intros. 
+  mgo_. subst. inv H. inv H0.
+  relax_apply insertA_pessim_. eauto.
+  cbn.
+  intros y n h. lia.
+Qed.
+
+Definition sizeT {a} ( x : T a) : nat := 
+  match x with 
+  | Thunk v => 1
+  | Undefined => 0
+  end.
+
+Definition insertSize : T (listA nat) -> nat := sizeAX sizeT 0.
+
+(* I don't know how to give an optimistic specification of insertA.
+   We don't know how many of the list elements need to be evaluated 
+   when we insert. *)
+Theorem insertA_prefix_cost : forall x (xsA : (listA nat)) n,
+    1 <= n <= sizeX' 0 xsA ->
+    (insertA_ x xsA) [[ fun zsA cost => n + 1 = sizeX' 0 zsA /\ cost <= 2 * n ]].
+Proof.
+  intro x.
+  induction xsA; mgo_list.
+Abort.
+
+(* Demand function for [insertA]. 
+   The input list needs to be forced only as long as its elements are <= x. 
+*)
+Fixpoint insertD_ (x:nat) (xs: list nat)  (outD : listA nat) : Tick (T (listA nat)) :=
+  match xs, outD with 
+  | nil, _ => Tick.ret (Thunk NilA)
+  | y :: ys, ConsA zD zsD => 
+     Tick.tick >>
+     if Nat.leb x y then 
+       Tick.tick >>
+       let+ ysD := thunkD (insertD_ x ys) zsD in
+       Tick.ret (Thunk (ConsA (Thunk y) ysD))
+     else 
+       Tick.ret zsD
+  | _ , _ => bottom
+  end.
+
+
+Definition insertD (x:nat) (xs: list nat) (outD : listA nat) : Tick (T nat * T (listA nat)) :=
+  Tick.tick >> Tick.tick >>
+  let+ ysD := insertD_ x xs outD in 
+  Tick.ret (Thunk x, ysD).
+
+Lemma insertD__approx (x : nat) (xs : list nat) (outD : _)
+  : outD `is_approx` insert x xs -> Tick.val (insertD_ x xs outD) `is_approx` xs.
+Proof.
+  revert outD; induction xs; cbn.
+  - intros; solve_approx.
+  - autorewrite with exact; intros. 
+    destruct (x <=? a) eqn:LE.
+    + inversion H; subst.    
+      inversion H4; subst; cbn. solve_approx.
+      specialize (IHxs _ H2). solve_approx.
+    + inversion H; subst. solve_approx.
+Qed.
+
+Lemma insertD_size x (xs : list nat) (outD : _)
+  : outD `is_approx` insert x xs ->
+    let ins := Tick.val (insertD_ x xs outD) in
+    (sizeX 0 ins) <= sizeX' 0 outD.
+Proof.
+  revert outD; induction xs; cbn; intros. 
+  inversion H; subst; cbn.
+  - destruct xs; lia. 
+  - destruct (x <=? a) eqn:L.
+    + inversion H; subst. cbn.
+      inversion H4. subst. cbn. auto.
+      subst. specialize (IHxs _ H2). cbn in IHxs.
+      cbn. destruct (Tick.val _) eqn:T. unfold sizeX in IHxs. lia. lia.
+    + inversion H. subst. cbn.
+      destruct xs0. simpl. auto. simpl. auto.
+Defined.
+
+
+Lemma insertD_spec x (xs : list nat) (outD : listA nat)
+  : outD `is_approx` insert x xs ->
+    forall xsD dcost, Tick.MkTick dcost xsD = insertD_ x xs outD ->
+    insertA (Thunk x) xsD [[ fun out cost => outD `less_defined` out /\ cost <= dcost ]].
+Proof.
+  unfold insertA.
+  revert outD; induction xs; cbn; intros * Hout *.
+  - unfold Tick.ret. intros h. inversion h. subst. 
+    mgo_.
+Admitted.
+
+End CaseStudyInsert.
+
+(* I'm not sure if we need these... *)
+
+(*
+Fixpoint selectA_ (l : listA nat) : M (option (T (listA nat) * nat)) :=
+  tick >>
+  match l with
+  | NilA => ret None
+  | ConsA x xs =>
+    forcing x (fun x =>
+    forcing xs (fun xs =>
+    let! o := selectA_ xs in
+    match o with
+    | None => ret (Some (Thunk NilA, x))
+    | Some (ys, y) =>
+      if x <? y then
+        ret (Some (Thunk (ConsA (Thunk y) ys), x))
+      else
+        ret (Some (Thunk (ConsA (Thunk x) ys), y))
+    end))
+  end.
+
+(* Invariant: n = length l. n is the decreasing argument. *)
+Fixpoint selectsortA (n : nat) (l : T (listA nat)) : M (listA nat) :=
+  tick >>
+  let! l := force l in
+  let! o := selectA_ l in
+  match n, o with
+  | S n, Some (ys, y) =>
+    let~ zs := selectsortA n ys in
+    ret (ConsA (Thunk y) zs)
+  | _, _ => ret NilA
+  end.
+
+Parameter selectsort : forall (l : list nat), list nat.
+
+Lemma selectsortA_cost {l n}
+  : n = length l ->
+    forall (d : listA nat), d `is_approx` exact (selectsort l) ->
+    let m := sizeX' 1 d in
+    selectsortA n (exact l) [[ fun sorted cost => d `less_defined` sorted /\ cost <= m * (length l + 1) ]].
+Proof.
+Admitted.
+
+Lemma selectsortA_cost' {l n}
+  : n = length l ->
+    forall (d : listA nat), d `is_approx` exact (selectsort l) ->
+    exists (lA : T (listA nat)), lA `is_approx` l /\
+    let m := sizeX' 1 d in
+    selectsortA n lA [[ fun sorted cost => d `less_defined` sorted /\ cost <= m * (length l + 1) ]].
+Proof.
+Admitted.
+
+*)
