src/MergeSort.v
@@ -1,0 +1,101 @@
+From Coq Require Import List Arith Psatz.
+
+From Clairvoyance Require Import Core Approx List ListA Tick.
+
+Import ListNotations.
+Import Tick.Notations.
+
+(* Now, what if we did the same but with mergesort *)
+
+(* MergeSort and its attendent functions as given by Software Foundations *) 
+
+Fixpoint split {X:Type} (l:list X) : (list X * list X) :=
+  match l with
+  | [] => ([],[])
+  | [x] => ([x],[])
+  | x1 :: x2 :: l' =>
+    let (l1,l2) := split l' in
+    (x1 :: l1, x2 :: l2)
+  end.
+
+Fixpoint merge l1 l2 n :=
+  match l1, l2, n with
+  | _, _, 0 => []
+  | [], _, _ => l2
+  | _, [], _ => l1
+  | a1::l1', a2::l2', S n =>
+      if a1 <=? a2 then a1 :: merge l1' l2 n else a2 :: merge l1 l2' n
+  end.
+
+(* We swapped this to use fuel instead of well-founded induction *)
+Fixpoint mergesort' (l: list nat) (n : nat) : list nat :=
+  match n, l with
+  | 0, _ => [] (* Ran out of fuel *)
+  | _, [] => []
+  | _, [x] => [x]
+  | S n, _ => let (l1,l2) := split l in 
+              merge (mergesort' l1 n) (mergesort' l2 n) (length l)
+  end.
+
+Definition mergesort (l : list nat) : list nat :=
+  mergesort' l (length l).
+
+(* Demand functions for split/merge/mergesort *)
+
+Definition thunkTupleD {a b} `{Bottom b} (f : a * a -> b) (x : T a * T a) (p : a) : b :=
+  match x with
+  | (Thunk x1, Thunk x2) => f (x1, x2)
+  | (Thunk x1, Undefined) => f (x1, p)
+  | (Undefined, Thunk x2) => f (p, x2)
+  | (Undefined, Undefined) => bottom
+  end.
+
+Fixpoint splitD {a : Type} (xs : list a) (outD : listA a * listA a) : Tick (T (listA a)) :=
+  Tick.tick >>
+  match xs, outD with
+  | [], _ => Tick.ret (Thunk NilA)
+  | [x], _ => Tick.ret (Thunk (ConsA (Thunk x) (Thunk NilA)))
+  | x :: x' :: xs, (ConsA zD zsD, ConsA zD' zsD') =>
+    Tick.tick >>
+    let+ xsD := thunkTupleD (splitD xs) (zsD, zsD') (ConsA Undefined Undefined) in
+    Tick.ret (Thunk (ConsA zD (Thunk (ConsA zD' xsD))))
+  | _, _ => bottom
+  end.
+
+(* Compute splitD [1;2;3;4;5;6;7;8] (exact [1;3;5;7], exact [2;4;6;8]). *)
+
+Fixpoint mergeD (xs ys : list nat) (outD : listA nat) : Tick (T (listA nat) * T (listA nat)) :=
+  Tick.tick >>
+  match xs, ys, outD with
+  | [], _, _ => Tick.ret (Thunk NilA, Undefined)
+  | _, [], _ => Tick.ret (Undefined, Thunk NilA)
+  | x :: xs, y :: ys, ConsA zD (Thunk (ConsA zD' zsD)) =>
+    Tick.tick >>
+    let+ (xsD, ysD) := thunkD (mergeD xs ys) zsD in
+    Tick.ret (Thunk (ConsA zD xsD), Thunk (ConsA zD' ysD))
+  | _, _, _ => bottom
+  end.
+
+Fixpoint mergesortD' (l : list nat) (n : nat) (outD : listA nat) : Tick (T (listA nat)) :=
+  Tick.tick >>
+  match l, outD, n with
+  | _, _, 0 => Tick.ret Undefined
+  | [], _, _ => Tick.ret (Thunk NilA)
+  | [x], _, _ => Tick.ret (Thunk (ConsA (Thunk x) (Thunk NilA)))
+  | _ :: _, ConsA _ _, S n =>
+    let (xs, ys) := split l in
+    let+ (mxsD, mysD) := mergeD (mergesort xs) (mergesort ys) outD in
+    let+ xsD := thunkD (mergesortD' xs n) mxsD in
+    let+ ysD := thunkD (mergesortD' ys n) mysD in
+    let+ lD := thunkTupleD (splitD l) (xsD, ysD) (ConsA Undefined Undefined) in
+    Tick.ret lD
+  | _, _, _ => bottom
+  end.
+
+Definition merge_sortD (l : list nat) (outD : listA nat) : Tick (T (listA nat)) :=
+  mergesortD' l (length l) outD.
+
+(* Long-term goal:
+   show that   head (selection_sort xs)   in O(n)
+   (also could be merge_sort) *)
+
