src/SelectionSort.v
@@ -1,0 +1,128 @@
+From Coq Require Import List Arith Psatz.
+
+From Clairvoyance Require Import Core Approx List ListA Tick Misc.
+
+Import ListNotations.
+Import Tick.Notations.
+
+(* Select and selsort as given by Software Foundations Chapter 3 *)
+Fixpoint select (x: nat) (l: list nat) : nat * list nat :=
+  match l with
+  | [] => (x, [])
+  | h :: t =>
+    if x <=? h
+    then let (j, l') := select x t in (j, h :: l')
+    else let (j, l') := select h t in (j, x :: l')
+  end.
+
+Fixpoint selection_sort (l : list nat) (n : nat) : list nat :=
+  match l, n with
+  | _, 0 => [] (* ran out of fuel *)
+  | [], _ => []
+  | x :: r, S n' => let (y, r') := select x r in y :: selection_sort r' n'
+end.
+
+(* The entire list must be forced to select smallest element *)
+Definition selectD (x : nat) (xs : list nat) (outD : listA nat) : Tick (T (listA nat)) :=
+  Tick.MkTick (1 + length xs) (exact (x::xs)).
+
+(* The entire list is forced one selection at a time*)
+Fixpoint selection_sortD (xs : list nat) (outD : listA nat) : Tick (T (listA nat)) :=
+  Tick.tick >>
+  match xs, outD with
+  | [], _ => Tick.ret (Thunk NilA)
+  | x :: xs', ConsA zD zsD =>
+    let+ _ := thunkD (selection_sortD xs') zsD in
+    let+ xsD := selectD x xs' (exact xs) in
+    Tick.ret xsD (* We invariably force the entire input list *)
+  | _, _ => bottom
+  end.
+
+Lemma sort_produces_element (n : nat) (x : nat) (xs : list nat) :
+  selection_sort (x :: xs) (S n) = fst (select x xs) :: selection_sort (snd (select x xs)) n.
+Proof.
+  simpl. destruct (select x xs). simpl. reflexivity.
+Qed.
+
+Definition head_def {a} (xs : list a) (d : a) : a :=
+  match xs with
+  | [] => d
+  | x :: _ => x
+  end.
+
+(* We force the empty list or the first element only *)
+Definition headD {a} (xs : list a) (d : a) (outD : a) : Tick (T (listA a)) :=
+  Tick.tick >>
+  match xs with
+  | [] => Tick.ret (Thunk NilA)
+  | x :: _ => Tick.ret (Thunk (ConsA (Thunk x) (Undefined)))
+  end.
+
+Definition head_selection_sortD (xs : list nat) (outD : nat) : Tick (T (listA nat)) :=
+  let+ list_headD := headD (selection_sort xs (length xs)) 0 outD in
+  let+ xsD := thunkD (selection_sortD xs) list_headD in
+  Tick.ret xsD.
+
+Lemma head_selection_sortD_cost (xs : list nat) (outD : nat) :
+  outD `is_approx` head_def (selection_sort xs (length xs)) 0 ->
+  forall xsA, xsA = Tick.val (head_selection_sortD xs outD) ->
+  Tick.cost (head_selection_sortD xs outD) <= length xs + 2.
+Proof.
+  intros. rewrite H. destruct xs.
+  - simpl. lia.
+  - unfold head_selection_sortD.
+    assert (H1 : length (n :: xs) = S (length xs)). auto. rewrite H1.
+    rewrite sort_produces_element. simpl. lia.
+Qed.
+
+Definition take_selection_sortD (n : nat) (xs : list nat) (outD : listA nat) :
+  Tick (T (listA nat)) :=
+  let+ list_takeD := takeD n (selection_sort xs (length xs)) outD in
+  let+ xsD := thunkD (selection_sortD xs) list_takeD in
+  Tick.ret xsD.
+
+Lemma selection_sortD_cost (xs : list nat) (outD : listA nat) :
+  Tick.cost (selection_sortD xs outD) <= (sizeX' 1 outD) * (length xs + 2).
+Proof.
+  intros. generalize dependent xs. induction outD;
+  intro; destruct xs; simpl; try rewrite IHoutD; lia.
+Qed.
+
+Lemma headD_demand {a} (xs : list a) (d : a) (outD : a) : 
+  sizeX 1 (Tick.val (headD xs d outD)) = 1.
+Proof.
+  destruct xs; reflexivity.
+Qed.
+
+Theorem head_selection_sortD_cost' (xs : list nat) (outD : nat) :
+  Tick.cost (head_selection_sortD xs outD) <= length xs + 3.
+Proof.
+  unfold head_selection_sortD. unfold Tick.bind. simpl.
+  unfold thunkD. destruct (selection_sort xs (length xs)); simpl;
+  rewrite selection_sortD_cost; simpl; lia.
+Qed.
+
+Lemma takeD_demand {a} (n : nat) (xs : list a) (outD : listA a) :
+  sizeX 1 (Tick.val (takeD n xs outD)) <= sizeX' 1 outD.
+Proof.
+  generalize dependent n. generalize dependent xs.
+  induction outD; intros;
+  destruct n; destruct xs; simpl; try lia.
+  destruct (Tick.val (takeD n xs outD)) eqn : E; try lia.
+  apply le_n_S. assert (H' : sizeX' 1 x = sizeX 1 (Thunk x)). { auto. }
+  rewrite H'. symmetry in E. rewrite E. apply IHoutD.
+Qed.
+
+Theorem take_selection_sortD_cost (n : nat) (xs : list nat) (outD : listA nat) :
+  Tick.cost (take_selection_sortD n xs outD) <= (sizeX' 1 outD) * (length xs + 2) + n + 1.
+Proof.
+  unfold take_selection_sortD. unfold Tick.bind. 
+  simpl. rewrite takeD_cost. unfold thunkD. 
+  destruct (Tick.val (takeD n (selection_sort xs (length xs)) outD)) eqn:  E.
+  - assert (H : sizeX' 1 x = sizeX 1 (Thunk x)). { reflexivity. }
+    symmetry in E. rewrite E in H.
+    rewrite selection_sortD_cost. rewrite H. rewrite takeD_demand. lia.
+  - simpl. lia.
+Qed.
+
+
